bigStep broken in two (success and fail)

biglir.v
@@ -18,19 +18,12 @@ Reserved Notation "m '/' e ==> m1 '/' e1"
 Reserved Notation "m '/' e ==> 'fail'"
 (at level 40, e at level 39).
 
-Inductive bigStep : Mem -> IRE -> Mem -> option IRE -> Prop :=
+Inductive bigStep : Mem -> IRE -> Mem -> IRE -> Prop :=
 | BStValue : forall m e, Value e -> m / e ==> m / e
 | BStPlus : forall m e1 m' n1 e2 m'' n2,
     m / e1 ==> m' / IRENum n1 ->
     m'/ e2 ==> m'' / IRENum n2 ->
     m / IREPlus e1 e2 ==> m'' / IRENum (n1 + n2)
-| BStPlus1F : forall m e1 e2,
-    m / e1 ==> fail ->
-    m / IREPlus e1 e2 ==> fail
-| BStPlus2F : forall m e1 m' n1 e2,
-    m / e1 ==> m' / IRENum n1 ->
-    m' / e2 ==> fail ->
-    m / IREPlus e1 e2 ==> fail
 | BStCstr : forall m m' free,
     (free, m') = fresh m ->
     m / IRECnst ==> m' / IREAddr free
@@ -39,6 +32,38 @@ Inductive bigStep : Mem -> IRE -> Mem -> option IRE -> Prop :=
     m'/ e2 ==> m'' / idx ->
     v = query a idx m'' ->
     m / IREGet e1 e2 ==> m'' / v
+| BStSet : forall m e1 m' a e2 m'' idx m''' e3 val,
+    m / e1 ==> m' / IREAddr a ->
+    m'/ e2 ==> m'' / idx ->
+    m''/ e3 ==> m''' / val ->
+    m / IRESet e1 e2 e3 ==> Update a (ToIndex idx) val m''' / val
+| BStLet : forall m exp m' v1 var t body m'' res,
+     m / exp ==> m' / v1 ->
+     m' / ([var := v1] body) ==> m'' / res ->
+     m / IRELet var t exp body ==> m'' / res
+| BStFunapp : forall m e1 m' var body e2 m'' v2 m''' res,
+    m / e1 ==> m' / IREFun var body ->
+    m' / e2 ==> m'' / v2 ->
+    m'' / ([var := v2] body) ==> m''' / res ->
+    m / IREFunApp e1 e2 ==> m''' / res
+| BStBox : forall m e m' e' t,
+    m / e ==> m' / e' ->
+    m / IREBox t e ==> m' / IREBox t e'
+| BStUnbox : forall m e m' t e',
+    m / e ==> m' / IREBox t e' ->
+    m / IREUnbox t e ==> m' / e'
+
+where "m / e ==> m1 / e1" := (bigStep m e m1 e1)
+.
+
+Inductive bigStepF : Mem -> IRE -> Prop :=
+| BStPlus1F : forall m e1 e2,
+    m / e1 ==> fail ->
+    m / IREPlus e1 e2 ==> fail
+| BStPlus2F : forall m e1 m' n1 e2,
+    m / e1 ==> m' / IRENum n1 ->
+    m' / e2 ==> fail ->
+    m / IREPlus e1 e2 ==> fail
 | BStGet1F : forall m e1 e2,
     m / e1 ==> fail ->
     m / IREGet e1 e2 ==> fail
@@ -46,11 +71,6 @@ Inductive bigStep : Mem -> IRE -> Mem -> option IRE -> Prop :=
     m / e1 ==> m' / IREAddr a ->
     m' / e2 ==> fail ->
     m / IREGet e1 e2 ==> fail
-| BStSet : forall m e1 m' a e2 m'' idx m''' e3 val,
-    m / e1 ==> m' / IREAddr a ->
-    m'/ e2 ==> m'' / idx ->
-    m''/ e3 ==> m''' / val ->
-    m / IRESet e1 e2 e3 ==> Update a (ToIndex idx) val m''' / val
 | BStSet1F : forall m e1 e2 e3,
     m / e1 ==> fail ->
     m / IRESet e1 e2 e3 ==> fail
@@ -63,10 +83,6 @@ Inductive bigStep : Mem -> IRE -> Mem -> option IRE -> Prop :=
     m'/ e2 ==> m'' / IRENum idx ->
     m''/ e3 ==> fail ->
     m / IRESet e1 e2 e3 ==> fail
-| BStLet : forall m exp m' v1 var t body m'' res,
-     m / exp ==> m' / v1 ->
-     m' / ([var := v1] body) ==> m'' / res ->
-     m / IRELet var t exp body ==> m'' / res
 | BStLet1F : forall m exp var t body,
      m / exp ==> fail ->
      m / IRELet var t exp body ==> fail
@@ -74,11 +90,6 @@ Inductive bigStep : Mem -> IRE -> Mem -> option IRE -> Prop :=
      m / exp ==> m' / v1 ->
      m' / ([var := v1] body) ==> fail ->
      m / IRELet var t exp body ==> fail
-| BStFunapp : forall m e1 m' var body e2 m'' v2 m''' res,
-    m / e1 ==> m' / IREFun var body ->
-    m' / e2 ==> m'' / v2 ->
-    m'' / ([var := v2] body) ==> m''' / res ->
-    m / IREFunApp e1 e2 ==> m''' / res
 | BStFunapp1F : forall m e1 e2,
     m / e1 ==> fail ->
     m / IREFunApp e1 e2 ==> fail
@@ -91,15 +102,9 @@ Inductive bigStep : Mem -> IRE -> Mem -> option IRE -> Prop :=
     m' / e2 ==> m'' / v2 ->
     m'' / ([var := v2] body) ==> fail ->
     m / IREFunApp e1 e2 ==> fail
-| BStBox : forall m e m' e' t,
-    m / e ==> m' / e' ->
-    m / IREBox t e ==> m' / IREBox t e'
 | BStBox1F : forall m e t,
     m / e ==> fail ->
     m / IREBox t e ==> fail
-| BStUnbox : forall m e m' t e',
-    m / e ==> m' / IREBox t e' ->
-    m / IREUnbox t e ==> m' / e'
 | BStUnboxF : forall m e m' t t' e',
     m / e ==> m' / IREBox t e' ->
     t <> t' ->
@@ -108,9 +113,7 @@ Inductive bigStep : Mem -> IRE -> Mem -> option IRE -> Prop :=
     m / e ==> fail ->
     m / IREUnbox t e ==> fail
 
-
-where "m / e ==> m1 / e1" := (bigStep m e m1 (Some e1))
-  and "m / e ==> 'fail'" := (bigStep m e m None)
+where "m / e ==> 'fail'" := (bigStepF m e)
 .
 
 
@@ -125,7 +128,7 @@ Ltac splitAnd :=
 
 
 Lemma valueNormal : forall m e m' res,
-    bigStep m e m' res -> Value e -> m = m' /\ res = Some e.
+    bigStep m e m' res -> Value e -> m = m' /\ res = e.
 Proof.
   intros m e m' res HB HV.
   induction HB; inversion HV; subst; eauto using Value;
@@ -142,12 +145,8 @@ Lemma BPreservation : forall (m m' : Mem) e e' t,
 Proof.
   intros m m' e e' t Hst HMC HTy.
   remember MEmpty as Γ.
-  remember (Some e') as E'.
-  generalize dependent e'.
   generalize dependent t.
-  induction Hst; intros ? HTy ? HE';
-  (* impossible cases *)
-  inversion HE'; subst;
+  induction Hst; intros ? HTy;
   (* apply type judgment and break 'and's *)
   inversion HTy; subst; split;
   (* instantiate induction hypotheses when possible *)
@@ -155,7 +154,7 @@ Proof.
   | [ HM : mem_correct ?M,
       HT : _ |= ?E : _,
       IH : mem_correct ?M -> _ -> _ |= ?E : _ -> _ |- _] =>
-        specialize (IH HM _ HT _ eq_refl) as [? [? ?]]
+        specialize (IH HM _ HT) as [? [? ?]]
   end;
   eauto using IRTyping,Value,mem_correct_fresh,mem_correct_update;
   (* handle substitutions inside FUN (not pretty yet) *)
@@ -236,7 +235,7 @@ Proof.
   end;
   (* extract equalities from injections *)
   repeat match goal with
-  | [H: Some _ = Some _ |- _] => injection H as H; subst
+  | [H: Some _ = Some _ |- _] => idtac H; injection H as H; subst
   end;
   (* clear useless equalities *)
   repeat match goal with | [H: ?E = ?E |- _] => clear H end;
@@ -245,14 +244,13 @@ Proof.
   try match goal with
     |[H: ?E = query _ _ _ |- _] =>
         assert (HC: Value E) by (rewrite H; apply HM); inversion HC
-    end;
-  (* queries being complex values (fun and lambdas which must be
+    end; subst.
+  - (* queries being complex values (fun and lambdas which must be
      broken to extract some equalities *)
-  (
-    eapply valueNormal in HB as [? HB1]; eauto using Value;
-    inversion HB1; subst;
-    eapply BStGet; eauto using bigStep,Value; congruence
-  ).
+    eapply valueNormal in HB as [? ?]; subst; trivial;
+    eapply BStGet; eauto using bigStep, Value; congruence.
+  - inversion H3; subst.
+    eapply BStSet; eauto using bigStep, Value; congruence.
 Qed.
 
 
@@ -341,17 +339,15 @@ Theorem bigSmall : forall m e t m' e',
     m / e -->* m' / e'.
 Proof.
   intros m e t m' e' HM ? HSt.
-  remember (Some e') as E'.
-  generalize dependent e'.
   generalize dependent t.
-  induction HSt; intros ? HTy ? Heq; inversion Heq; clear Heq; subst;
+  induction HSt; intros ? HTy;
   inversion HTy; subst;
   repeat memC;
   repeat match goal with
     [ IH: mem_correct ?M  -> _ -> IRTyping _ ?E _ -> _,
       HM: mem_correct ?M,
       HT: IRTyping _ ?E _ |- _] =>
-        specialize (IH HM _ HT _ eq_refl)
+        specialize (IH HM _ HT)
     end;
     eauto using multistep.
   - eauto 6 using mPlus1, mPlus2, Value, multistep1, step, multiRefl.
@@ -392,11 +388,8 @@ Theorem bigDyn : forall e t m e' m',
 Proof.
   intros e t m e' m' HB HTy HM.
   remember MEmpty as Γ eqn:Heq.
-  remember (Some e') as E'.
-  generalize dependent e'.
   generalize dependent t.
-  induction HB; intros ? HTy ? Heq1;
-  inversion Heq1; clear Heq1;
+  induction HB; intros ? HTy;
   inversion Heq; inversion HTy; subst; simpl;
   try match goal with [H : Value _ |- _] => inversion H end;
   repeat memC;
@@ -405,13 +398,10 @@ Proof.
   eauto using Value,BStValue,dynValue,dynFresh,bigStep;
   repeat match goal with
     | [ MC: mem_correct ?M,
-        HT: MEmpty |= ?E : _ |- _] =>
-      match goal with
-      | [ IH: mem_correct M -> forall _, MEmpty |= E : _ ->
-        forall _, Some ?E' = Some _ -> _
+        HT: MEmpty |= ?E : _,
+        IH: mem_correct ?M -> forall _, MEmpty |= ?E : _ -> _
          |- _] =>
-        specialize (IH MC _ HT E' eq_refl); simpl in IH
-      end
+        specialize (IH MC _ HT); simpl in IH
     end; eauto using bigStep.
   - rewrite dynQuery. eauto using bigStep.
   - rewrite DynIndex. eauto using bigStep.
